concurrency/scache/SimpleCacheSM.i.dfy
@@ -1,0 +1,103 @@
+include "../framework/DiskSSM.s.dfy"
+include "CacheTypes.i.dfy"
+
+module SimpleCacheStateMachine refines StateMachine(CrashAsyncIfc(CacheIfc)) {
+  import opened CacheTypes
+
+  datatype Entry =
+    | Empty
+    | Reading(disk_idx: nat)
+    | Full(disk_idx: nat, data: seq<byte>)
+    | Dirty(disk_idx: nat, data: seq<byte>)
+    | Writeback(disk_idx: nat, data: seq<byte>)
+  )
+
+  datatype Variables = Variables(
+    entries: map<nat, Entry>,
+    write_reqs: map<nat, seq<byte>>,
+    write_resps: set<nat>,
+    read_reqs: set<nat>,
+    read_resps: map<nat, seq<byte>>,
+    tickets: map<RequestId, IOIfc.Input>,
+    stubs: map<RequestId, IOIfc.Output>
+    disk: map<nat, seq<byte>>
+  )
+
+  predicate StartRead(s: Variables, s': Variables, op: IOIfc.Op, cache_idx: nat, disk_idx: nat) {
+    && op.InternalOp?
+    && cache_idx in s.entries
+    && s.entries[cache_idx].Empty?
+    && (forall i | i in entries :: entries[i].status != Empty ==>
+          entries[i].disk_idx != disk_idx)
+    && s' == s
+      .(entries := s.entries[cache_idx := Reading(disk_idx)])
+      .(read_reqs := s.read_reqs + {disk_idx})
+  }
+
+  predicate FinishRead(s: Variables, s': Variables, op: IOIfc.Op, cache_idx: nat, disk_idx: nat) {
+    && op.InternalOp?
+    && cache_idx in s.entries
+    && disk_idx in s.read_resps
+    && s.entries[cache_idx].Reading?
+    && s.entries[cache_idx].disk_idx == disk_idx
+    && s' == s
+      .(entries := s.entries[cache_idx := Clean(disk_idx, s.read_resps[disk_idx].data)])
+      .(read_resps := s.read_resps - {disk_idx})
+  }
+
+  predicate MakeDirty(s: Variables, s': Variables, op: IOIfc.Op, cache_idx: nat) {
+    && op.InternalOp?
+    && cache_idx in s.entries
+    && s.entries[cache_idx].Clean?
+    && s' == s.(entries := s.entries[cache_idx := Dirty(s.entries[cache_idx].disk_idx, s.entries[cache_idx].data))
+  }
+
+  predicate StartWriteback(s: Variables, s': Variables, op: IOIfc.Op, cache_idx: nat, disk_idx: nat) {
+    && op.InternalOp?
+    && cache_idx in s.entries
+    && s.entries[cache_idx].Dirty?
+    && s.entries[cache_idx].disk_idx == disk_idx
+    && s' == s
+        .(entries := s.entries[cache_idx] := Writeback(s.entries[cache_idx].disk_idx, s.entries[cache_idx].data))
+        .(write_reqs := s.write_reqs[disk_idx := s.entries[cache_idx].data])
+  }
+
+  predicate FinishWriteback(s: Variables, s': Variables, op: IOIfc.Op, cache_idx: nat, disk_idx: nat) {
+    && op.InternalOp?
+    && cache_idx in s.entries
+    && s.entries[cache_idx].Writeback?
+    && s.entries[cache_idx].disk_idx == disk_idx
+    && s' == s
+        .(entries := s.entries[cache_idx] := Clean(s.entries[cache_idx].disk_idx, s.entries[cache_idx].data))
+        .(write_resps := s.write_resps - {disk_idx})
+  }
+
+  predicate Evict(s: Variables, s': Variables, op: IOIfc.Op, cache_idx: nat) {
+    && op.InternalOp?
+    && cache_idx in s.entries
+    && s.entries[cache_idx].Clean?
+    && s' == s
+        .(entries := s.entries[cache_idx := Empty])
+  }
+
+  predicate ProcessRead(s: Variables, s': Variables, op: IOIfc.Op, disk_idx: nat) {
+    && op.InternalOp?
+    && disk_idx in s.read_reqs
+    && disk_idx in s.disk
+    && s' == s
+        .(read_reqs := s.read_reqs - {disk_idx})
+        .(read_resps := s.read_resps[disk_idx := s.disk[disk_idx]])
+  }
+
+  predicate ProcessWrite(s: Variables, s': Variables, op: IOIfc.Op, disk_idx: nat) {
+    && op.InternalOp?
+    && disk_idx in s.write_reqs
+    && s' == s
+        .(write_reqs := s.write_reqs - {disk_idx})
+        .(write_resps := s.write_resps[disk_idx + {disk_idx}])
+        .(disk := s.disk[disk_idx := s.write_reqs[disk_idx].data])
+  }
+
+  predicate Crash(s: Variables, s': Variables, op: IOIfc.Op) {
+  }
+}
